CC/CaptureSet.lean
@@ -10,9 +10,9 @@ structure CaptureSet (n : Nat) (k : Nat) where
   rdr : Bool
   cap : Bool
 
-inductive SepDegree (n : Nat) where
-| elems : Finset (Fin n) -> SepDegree n
-| uniq : SepDegree n
+inductive SepDegree (n : Nat) (k : Nat) where
+| elems : Finset (BiFin n k) -> SepDegree n k
+| uniq : SepDegree n k
 
 def CaptureSet.rdrSet (C : CaptureSet n k) : CaptureSet n k :=
   { elems := {}, rdr := C.rdr, cap := false }
@@ -26,7 +26,7 @@ def CaptureSet.hasRdr (C : CaptureSet n k) : Prop :=
 def CaptureSet.hasCap (C : CaptureSet n k) : Prop :=
   C.cap = true
 
-def SepDegree.isUniq (D : SepDegree n) : Prop :=
+def SepDegree.isUniq (D : SepDegree n k) : Prop :=
   match D with
   | SepDegree.elems _ => false
   | SepDegree.uniq => true
@@ -48,150 +48,151 @@ instance : Singleton (BiFin n k) (CaptureSet n k) :=
 instance : Union (CaptureSet n k) :=
   ⟨fun s t => ⟨s.1 ∪ t.1, s.2 || t.2, s.3 || t.3⟩⟩ 
 
--- instance : EmptyCollection (CaptureSet n) :=
---   ⟨⟨{}, false, false⟩⟩
+instance : EmptyCollection (CaptureSet n k) :=
+  ⟨⟨{}, false, false⟩⟩
 
--- def SepDegree.mem (a : Fin n) (D : SepDegree n) :=
---   match D with
---   | SepDegree.elems xs => a ∈ xs
---   | SepDegree.uniq => False
+def SepDegree.mem (a : BiFin n k) (D : SepDegree n k) :=
+  match D with
+  | SepDegree.elems xs => a ∈ xs
+  | SepDegree.uniq => False
 
--- instance : Membership (Fin n) (SepDegree n) :=
---   ⟨fun a s => s.mem a⟩
+instance : Membership (BiFin n k) (SepDegree n k) :=
+  ⟨fun a s => s.mem a⟩
 
--- def SepDegree.singleton (x : Fin n) : SepDegree n :=
---   SepDegree.elems {x}
+def SepDegree.singleton (x : BiFin n k) : SepDegree n k :=
+  SepDegree.elems {x}
 
--- instance : Singleton (Fin n) (SepDegree n) :=
---   ⟨fun x => SepDegree.singleton x⟩
+instance : Singleton (BiFin n k) (SepDegree n k) :=
+  ⟨fun x => SepDegree.singleton x⟩
 
 -- -- instance : Union (SepDegree n) :=
 -- --   ⟨fun s t => ⟨s.1 ∪ t.1, s.2 || t.2⟩⟩
 
--- instance : EmptyCollection (SepDegree n) :=
---   ⟨SepDegree.elems {}⟩
+instance : EmptyCollection (SepDegree n k) :=
+  ⟨SepDegree.elems {}⟩
 
--- def CaptureSet.rename (C : CaptureSet n1) (f : VarMap n1 n2) : CaptureSet n2 :=
---   ⟨C.elems.image f, C.rdr, C.cap⟩
+def CaptureSet.rename (C : CaptureSet n1 k1) (f : BVarMap n1 k1 n2 k2) : CaptureSet n2 k2 :=
+  ⟨C.elems.image f, C.rdr, C.cap⟩
 
--- def SepDegree.rename (C : SepDegree n1) (f : VarMap n1 n2) : SepDegree n2 :=
---   match C with
---   | SepDegree.elems xs => SepDegree.elems (xs.image f)
---   | SepDegree.uniq => SepDegree.uniq
+def SepDegree.rename (C : SepDegree n1 k1) (f : BVarMap n1 k1 n2 k2) : SepDegree n2 k2 :=
+  match C with
+  | SepDegree.elems xs => SepDegree.elems (xs.image f)
+  | SepDegree.uniq => SepDegree.uniq
   
--- def CaptureSet.weaken_var (C : CaptureSet n) : CaptureSet n.succ :=
---   C.rename weaken_map
+def CaptureSet.weaken_var (C : CaptureSet n k) : CaptureSet n.succ k :=
+  C.rename weaken_bmap
 
--- def SepDegree.weaken_var (D : SepDegree n) : SepDegree n.succ :=
---   D.rename weaken_map
+def SepDegree.weaken_var (D : SepDegree n k) : SepDegree n.succ k :=
+  D.rename weaken_bmap
 
--- theorem singleton_val (x : Fin n) :
---   ({x} : CaptureSet n).1 = {x} := rfl
+theorem singleton_val (x : BiFin n k) :
+  ({x} : CaptureSet n k).1 = {x} := rfl
 
--- @[simp]
--- theorem rename_singleton (x : Fin n) (f : VarMap n n') :
---   CaptureSet.rename {x} f = {f x} := by
---   simp [CaptureSet.rename]
---   aesop
+@[simp]
+theorem rename_singleton (x : BiFin n k) (f : BVarMap n k n' k') :
+  CaptureSet.rename {x} f = {f x} := by
+  simp [CaptureSet.rename]
+  aesop
 
--- @[simp]
--- theorem rename_empty (f : VarMap n n') :
---   CaptureSet.rename ∅ f = ∅ := by
---   simp [CaptureSet.rename]
---   aesop
+@[simp]
+theorem rename_empty (f : BVarMap n k n' k') :
+  CaptureSet.rename ∅ f = ∅ := by
+  simp [CaptureSet.rename]
+  aesop
 
--- @[simp]
--- theorem SepDegree.rename_empty :
---   SepDegree.rename {} f = {} := by
---   simp [SepDegree.rename]
---   aesop
+@[simp]
+theorem SepDegree.rename_empty :
+  SepDegree.rename {} f = {} := by
+  simp [SepDegree.rename]
+  aesop
 
--- theorem mem_def {x : Fin n} {C : CaptureSet n} : x ∈ C ↔ x ∈ C.1 := Iff.rfl
+theorem mem_def {x : BiFin n k} {C : CaptureSet n k} : x ∈ C ↔ x ∈ C.1 := Iff.rfl
 
--- theorem singleton_def {x : Fin n} : ({x} : CaptureSet n).elems = {x} := rfl
+theorem singleton_def {x : BiFin n k} : ({x} : CaptureSet n k).elems = {x} := rfl
 
--- theorem mem_rename_of_mem (f : VarMap n1 n2) {C : CaptureSet n1} (h : x ∈ C) : f x ∈ C.rename f := by
---   unfold CaptureSet.rename
---   simp [mem_def]
---   aesop
+theorem mem_rename_of_mem 
+  (f : BVarMap n1 k1 n2 k2) {C : CaptureSet n1 k1} (h : x ∈ C) : f x ∈ C.rename f := by
+  unfold CaptureSet.rename
+  simp [mem_def]
+  aesop
 
--- instance decidableMem (x : Fin n) (C : CaptureSet n) : Decidable (x ∈ C) :=
---   Finset.decidableMem _ _
+instance decidableMem (x : BiFin n k) (C : CaptureSet n k) : Decidable (x ∈ C) :=
+  Finset.decidableMem _ _
 
--- @[simp]
--- theorem mem_rename {C : CaptureSet n} :
---   y ∈ C.rename f ↔ ∃ x ∈ C, f x = y := by
---   simp only [CaptureSet.rename, mem_def]
---   aesop
+@[simp]
+theorem mem_rename {C : CaptureSet n k} :
+  y ∈ C.rename f ↔ ∃ x ∈ C, f x = y := by
+  simp only [CaptureSet.rename, mem_def]
+  aesop
 
--- theorem union_def {C1 C2 : CaptureSet n} : 
---   C1 ∪ C2 = ⟨C1.1 ∪ C2.1, C1.2 || C2.2, C1.3 || C2.3⟩ := rfl
+theorem union_def {C1 C2 : CaptureSet n k} : 
+  C1 ∪ C2 = ⟨C1.1 ∪ C2.1, C1.2 || C2.2, C1.3 || C2.3⟩ := rfl
 
--- @[simp]
--- theorem CaptureSet.rename_id : ∀ {C : CaptureSet n},
---   C.rename id = C := by
---   introv
---   simp [CaptureSet.rename]
+@[simp]
+theorem CaptureSet.rename_id : ∀ {C : CaptureSet n k},
+  C.rename id = C := by
+  introv
+  simp [CaptureSet.rename]
 
--- @[simp]
--- theorem SepDegree.rename_id : ∀ {D : SepDegree n},
---   D.rename id = D := by
---   introv
---   cases D <;> simp [SepDegree.rename]
+@[simp]
+theorem SepDegree.rename_id : ∀ {D : SepDegree n k},
+  D.rename id = D := by
+  introv
+  cases D <;> simp [SepDegree.rename]
 
--- @[simp]
--- theorem CaptureSet.rename_id' : ∀ {C : CaptureSet n},
---   C.rename (fun x => x) = C := by
---   introv
---   simp [CaptureSet.rename]
+@[simp]
+theorem CaptureSet.rename_id' : ∀ {C : CaptureSet n k},
+  C.rename (fun x => x) = C := by
+  introv
+  simp [CaptureSet.rename]
 
--- theorem CaptureSet.rename_comp {C : CaptureSet n1} {f1 : VarMap n1 n2} {f2 : VarMap n2 n3} :
---   (C.rename f1).rename f2 = C.rename (f2.comp f1) := by
---   unfold VarMap.comp
---   simp [CaptureSet.rename, Finset.image_image]
+theorem CaptureSet.rename_comp {C : CaptureSet n1 k1} {f1 : BVarMap n1 k1 n2 k2} {f2 : BVarMap n2 k2 n3 k3} :
+  (C.rename f1).rename f2 = C.rename (f2.comp f1) := by
+  unfold BVarMap.comp
+  simp [CaptureSet.rename, Finset.image_image]
 
--- theorem SepDegree.rename_comp {D : SepDegree n1} {f1 : VarMap n1 n2} {f2 : VarMap n2 n3} :
---   (D.rename f1).rename f2 = D.rename (f2.comp f1) := by
---   unfold VarMap.comp
---   cases D <;> simp [SepDegree.rename, Finset.image_image]
+theorem SepDegree.rename_comp {D : SepDegree n1 k1} {f1 : BVarMap n1 k1 n2 k2} {f2 : BVarMap n2 k2 n3 k3} :
+  (D.rename f1).rename f2 = D.rename (f2.comp f1) := by
+  unfold BVarMap.comp
+  cases D <;> simp [SepDegree.rename, Finset.image_image]
 
--- theorem CaptureSet.rename_union {C1 C2 : CaptureSet n} :
---   (C1 ∪ C2).rename f = C1.rename f ∪ C2.rename f := by
---   simp [CaptureSet.rename, union_def, Finset.image_union]
+theorem CaptureSet.rename_union {C1 C2 : CaptureSet n k} :
+  (C1 ∪ C2).rename f = C1.rename f ∪ C2.rename f := by
+  simp [CaptureSet.rename, union_def, Finset.image_union]
 
--- def CaptureSet.open_var (C : CaptureSet n.succ) (z : Fin n) : CaptureSet n :=
---   C.rename (open_map z)
+def CaptureSet.open_var (C : CaptureSet n.succ k) (z : Fin n) : CaptureSet n k :=
+  C.rename (open_bmap z)
 
--- lemma CaptureSet.val_eq {C1 C2 : CaptureSet n} 
---   (h1 : C1.elems = C2.elems)
---   (h2 : C1.rdr = C2.rdr)
---   (h3 : C1.cap = C2.cap) :
---   C1 = C2 := 
---   by cases C1; cases C2; aesop
+lemma CaptureSet.val_eq {C1 C2 : CaptureSet n k} 
+  (h1 : C1.elems = C2.elems)
+  (h2 : C1.rdr = C2.rdr)
+  (h3 : C1.cap = C2.cap) :
+  C1 = C2 := 
+  by cases C1; cases C2; aesop
 
--- lemma CaptureSet.val_def :
---   ({ elems := xs, rdr := b1, cap := b2 } : CaptureSet n).elems = xs := rfl
+lemma CaptureSet.val_def :
+  ({ elems := xs, rdr := b1, cap := b2 } : CaptureSet n k).elems = xs := rfl
 
--- lemma CaptureSet.elems_val_eq {C1 C2 : CaptureSet n}
---   (he : C1 = C2) :
---   C1.elems = C2.elems := by aesop
+lemma CaptureSet.elems_val_eq {C1 C2 : CaptureSet n k}
+  (he : C1 = C2) :
+  C1.elems = C2.elems := by aesop
 
--- lemma CaptureSet.cap_val_eq {C1 C2 : CaptureSet n}
---   (he : C1 = C2) :
---   C1.cap = C2.cap := by aesop
+lemma CaptureSet.cap_val_eq {C1 C2 : CaptureSet n k}
+  (he : C1 = C2) :
+  C1.cap = C2.cap := by aesop
 
--- @[simp]
--- lemma CaptureSet.cap_val_def :
---   ({ elems := xs, rdr := b1, cap := b2 } : CaptureSet n).cap = b2 := rfl
+@[simp]
+lemma CaptureSet.cap_val_def :
+  ({ elems := xs, rdr := b1, cap := b2 } : CaptureSet n k).cap = b2 := rfl
 
--- lemma CaptureSet.in_union_elems {C1 C2 : CaptureSet n}
---   (h : x ∈ (C1 ∪ C2).elems) :
---   x ∈ C1.elems ∨ x ∈ C2.elems := by
---   cases C1; cases C2
---   simp [union_def] at h
---   aesop
+lemma CaptureSet.in_union_elems {C1 C2 : CaptureSet n k}
+  (h : x ∈ (C1 ∪ C2).elems) :
+  x ∈ C1.elems ∨ x ∈ C2.elems := by
+  cases C1; cases C2
+  simp [union_def] at h
+  aesop
 
--- def CaptureSet.weaken_var1 (C : CaptureSet (Nat.succ n)) : CaptureSet n.succ.succ :=
+-- def CaptureSet.weaken_var1 (C : CaptureSet (Nat.succ n) k) : CaptureSet n.succ.succ k :=
 --   C.rename weaken_map.ext
 
 -- def SepDegree.weaken_var1 (D : SepDegree (Nat.succ n)) : SepDegree n.succ.succ :=
