CC/BiFin.lean
@@ -2,3 +2,17 @@
 inductive BiFin : Nat -> Nat -> Type where
 | injn : Fin n -> BiFin n k
 | injk : Fin k -> BiFin n k
+
+def BiFin.instDecEq (n k : Nat) : DecidableEq (BiFin n k)
+| injn i, injn j =>
+  match (decEq i j) with
+  | isTrue p => isTrue (congrArg injn p)
+  | isFalse p => isFalse (fun h => by cases h; apply p; rfl)
+| injk i, injk j =>
+  match (decEq i j) with
+  | isTrue p => isTrue (congrArg injk p)
+  | isFalse p => isFalse (fun h => by cases h; apply p; rfl)
+| injn i, injk j => isFalse (fun h => by cases h)
+| injk i, injn j => isFalse (fun h => by cases h)
+
+instance (n k : Nat) : DecidableEq (BiFin n k) := BiFin.instDecEq n k
